compose/Sem.v
@@ -21,19 +21,16 @@ Set Implicit Arguments.
 
 
 
-Definition Midx := nat.
-Definition Ohs := Midx -> option { oh: Type & oh }.
-Definition update Y (map: Midx -> Y) (x: Midx) (y: Y): Midx -> Y := fun n => if Nat.eq_dec x n then y else map x.
+Definition Ohs := Midx.t -> { oh: Type & oh }.
 
 Module Frame.
 
   Record t: Type := mk {
     ms: ModSem.t;
     st: ms.(ModSem.state); (* local state *)
-    midx: Midx;
   }.
 
-  Definition update_st (fr0: t) (st0: fr0.(ms).(ModSem.state)): t := (mk fr0.(ms) st0 fr0.(midx)).
+  Definition update_st (fr0: t) (st0: fr0.(ms).(ModSem.state)): t := (mk fr0.(ms) st0).
 
 End Frame.
 
@@ -44,19 +41,18 @@ Module Ge.
   (* NOTE: Ge.(snd) is not used in semantics. It seems it is just for convenience in meta theory *)
   Definition t: Type := (list ModSem.t * SkEnv.t).
 
-  (* TODO: remove redundancy? ms, midx *)
-  Inductive find_fptr_owner (ge: t) (fptr: val) (ms: ModSem.t) (midx: Midx): Prop :=
+  Inductive find_fptr_owner (ge: t) (fptr: val) (ms: ModSem.t): Prop :=
   | find_fptr_owner_intro
-      (MODSEM: List.nth_error (fst ge) midx = Some ms)
+      (MODSEM: List.find (fun ms0 => Midx.eqb ms.(ModSem.midx) ms0.(ModSem.midx)) (fst ge) = Some ms)
       if_sig
       (INTERNAL: Genv.find_funct ms.(ModSem.skenv) fptr = Some (Internal if_sig)).
 
   Inductive disjoint (ge: t): Prop :=
   | disjoint_intro
-      (DISJOINT: forall fptr ms0 ms1 midx0 midx1
-          (FIND0: ge.(find_fptr_owner) fptr ms0 midx0)
-          (FIND1: ge.(find_fptr_owner) fptr ms1 midx1),
-          ms0 = ms1 /\ midx0 = midx1).
+      (DISJOINT: forall fptr ms0 ms1
+          (FIND0: ge.(find_fptr_owner) fptr ms0)
+          (FIND1: ge.(find_fptr_owner) fptr ms1),
+          ms0 = ms1).
 
 End Ge.
 
@@ -82,17 +78,17 @@ Inductive step (ge: Ge.t): state -> trace -> state -> Prop :=
 | step_call
     fr0 frs args oh ohs0 ohs1 
     (AT: fr0.(Frame.ms).(ModSem.at_external) fr0.(Frame.st) oh args)
-    (OHS: ohs1 = update ohs0 fr0.(Frame.midx) (Some (existT id _ oh))):
+    (OHS: ohs1 = Midx.update ohs0 fr0.(Frame.ms).(ModSem.midx) (existT id _ oh)):
     step ge (State (fr0 :: frs) ohs0)
          E0 (Callstate args (fr0 :: frs) ohs1)
 
 | step_init
-    args frs ms midx st_init oh ohs
-    (MSFIND: ge.(Ge.find_fptr_owner) (Args.get_fptr args) ms midx)
-    (OH: ohs midx = Some (existT id _ oh))
+    args frs ms st_init oh ohs
+    (MSFIND: ge.(Ge.find_fptr_owner) (Args.get_fptr args) ms)
+    (OH: ohs ms.(ModSem.midx) = (existT id _ oh))
     (INIT: ms.(ModSem.initial_frame) oh args st_init):
     step ge (Callstate args frs ohs)
-         E0 (State ((Frame.mk ms st_init midx) :: frs) ohs)
+         E0 (State ((Frame.mk ms st_init) :: frs) ohs)
 
 | step_internal
     fr0 frs tr st0 ohs
@@ -103,8 +99,8 @@ Inductive step (ge: Ge.t): state -> trace -> state -> Prop :=
     fr0 fr1 frs retv st0 ohs0 ohs1 oh0 oh1
     (FINAL: fr0.(Frame.ms).(ModSem.final_frame) fr0.(Frame.st) oh0 retv)
     (AFTER: fr1.(Frame.ms).(ModSem.after_external) fr1.(Frame.st) oh1 retv st0)
-    (OHS: ohs1 = update ohs0 fr0.(Frame.midx) (Some (existT id _ oh0)))
-    (OH: ohs1 fr1.(Frame.midx) = Some (existT id _ oh1)):
+    (OHS: ohs1 = Midx.update ohs0 fr0.(Frame.ms).(ModSem.midx) (existT id _ oh0))
+    (OH: ohs1 fr1.(Frame.ms).(ModSem.midx) = (existT id _ oh1)):
     step ge (State (fr0 :: fr1 :: frs) ohs0)
          E0 (State (((Frame.update_st fr1) st0) :: frs) ohs1)
 .
@@ -127,16 +123,23 @@ Section SEMANTICS.
                                       end).
 
   Definition load_system (skenv: SkEnv.t): (ModSem.t * SkEnv.t) :=
-    (System.modsem skenv, (skenv_fill_internals skenv)).
+    (System.modsem Midx.ground skenv, (skenv_fill_internals skenv)).
 
-  Definition load_modsems (skenv: SkEnv.t): list ModSem.t := List.map ((flip Mod.modsem) skenv) p.
+  Definition load_modsems (skenv: SkEnv.t): list ModSem.t :=
+    Midx.map_with_midx (fun midx md => (Mod.modsem md midx skenv)) p.
 
   Definition load_genv (init_skenv: SkEnv.t): Ge.t :=
     let (system, skenv) := load_system init_skenv in
     (system :: (load_modsems init_skenv), init_skenv).
 
   Definition load_owned_heaps (ge: Ge.t): Ohs :=
-    List.nth_error (map (fun ms => (existT id _ ms.(ModSem.initial_owned_heap))) (fst ge))
+    fun midx =>
+      match List.find (fun ms => Midx.eqb midx ms.(ModSem.midx)) (fst ge) with
+      | Some ms => existT id _ ms.(ModSem.initial_owned_heap)
+      | _ => (@existT Type (fun _ => _) unit tt)
+      end
+      (* List.nth midx (map (fun ms => (existT id _ ms.(ModSem.initial_owned_heap))) (fst ge)) *)
+      (*                    (@existT Type (fun _ => _) unit tt) *)
   .
 
   (* Making dummy_module that calls main? => Then what is sk of it? Memory will be different with physical linking *)
